[TOC]

# Chapter 6: **Inner Product Spaces**

## _Exercise 1_

Suppose $w \in \\{v_1, \dots, v_m\\}^\perp$.
Let $v = \in \operatorname{span}(v_1, \dots, v_m)$.
We have that

$$
v = a_1 v_1 + \dots a_m v_m
$$

for some $a_1, \dots, a_m \in \mathbb{F}$.
Moreover

$$
\langle v, w \rangle = \langle a_1 v_1 + \dots a_m v_m, w \rangle = a_1 \langle v_1, w \rangle + \dots + a_m \langle v_m, w \rangle = 0.
$$

Thus $w \in (\operatorname{span}(v_1, \dots, v_m))^\perp$ and so $\\{v_1, \dots, v_m\\}^\perp \subset (\operatorname{span}(v_1, \dots, v_m))^\perp$.

Now suppose $w \in (\operatorname{span}(v_1, \dots, v_m))^\perp$.
Since each $v_j$ is in $\operatorname{span}(v_1, \dots, v_m)$, it follows that $w$ is orthogonal to each $v_j$.
Therefore $w \in \\{v_1, \dots, v_m\\}^\perp$ and thus $(\operatorname{span}(v_1, \dots, v_m))^\perp \subset \\{v_1, \dots, v_m\\}^\perp$.

## _Exercise 2_

Suppose $U^\perp = \\{0\\}$.
Since $V = U \oplus U^\perp$ (by 6.47), it follows that $U = V$.

Conversely, suppose $U = V$.
Then $U^\perp = V^\perp = \\{0\\}$.

## _Exercise 3_

By 6.31, we have $\operatorname{span}(u_1, \dots, u_m) = \operatorname{span}(e_1, \dots, e_m)$.
Therefore $e_1, \dots, e_m$ is indeed an orthonormal basis of $U$.
Clearly $\operatorname{span}(f_1, \dots, f_n) \subset U^\perp$ (because each of the $f$'s are orthogonal to the basis of $U$).
Moreover,

$$
\operatorname{dim} U^\perp = \operatorname{dim} V - \operatorname{dim} U = m + n - m = n.
$$

Hence $f_1, \dots, f_n$ is linearly independent list of length $\operatorname{dim} U^\perp$, that is, a basis of $U^\perp$.

## _Exercise 5_

Suppose $v \in V$.
By 6.47, we can write $v = u + w$, where $u \in U$ and $w \in U^\perp$.
Note that, by 6.51, $(U^\perp)^\perp = U$.
Thus $P_{U^\perp}v = w$, because $u \in (U^\perp)^\perp$.
Therefore

$$
P_{U^\perp}v = w = v - u = Iv - P_Uv = (I - P_U)v.
$$

Hence $P_{U^\perp} = I - P_U$.

## _Exercise 6_

Suppose $P_U P_W = 0$.
Then $\operatorname{range} P_W \subset \operatorname{null} P_U$.
However, 6.55 shows that $\operatorname{range} P_W = W$ and $\operatorname{null} P_U = U^\perp$.
Thus $W \subset U^\perp$, which implies that $\langle u, w \rangle = 0$ for all $u \in U$ and all $w \in W$.

Conversely, suppose $\langle u, w \rangle = 0$ for all $u \in U$ and all $w \in W$.
It follows that $W \subset U^\perp$.
Let $v \in V$.
By 6.47, we can write $v = w + u$, where $w \in W$ and $u \in W^\perp$.
Then

$$
P_U P_W v = P_Uw = 0.
$$

Where the last equality, follows from the fact that $W \subset U^\perp$.

## _Exercise 7_

Define $U = \operatorname{range} P$.
Suppose $u \in U$.
There exists $v \in V$ such that $Pv = u$.
Then

$$
u = Pv = P^2 v = P(Pv) = Pu.
$$

We've shown that $Pu = u$ for any $u \in U$.
Let $v \in V$.
By Exercise 4 in section 5B, we can write $v = u + w$ for some $u \in U$ and $w \in \operatorname{null} P$.
Note that $\operatorname{null} P \subset U^\perp$.
Thus

$$
Pv = P(u + w) = Pu = u = P_U(u + w) = P_Uv.
$$

Therefore $P = P_U$.

## _Exercise 9_

Suppose $U$ is invariant under $T$.
Let $v \in V$.
Then, by part (b) in 6.55, $P_U v \in U$, which implies that $T P_U v \in U$ (since $U$ is invariant under $T$), which implies that $P_U T P_U v = T P_U v$.
Thus $P_U T P_U = T P_U$.

Conversely, suppose $P_U T P_U = T P_U$.
Let $u \in U$.
Then

$$
T_U = T P_U u = P_U T P_U u \in U.
$$
Therefore $U$ is invariant under $T$.

## _Exercise 10_

Suppose $U$ and $U^\perp$ are both invariant under $T$.
Let $v \in V$.
Then $v = u + w$ for some $u \in U$ and $w \in U^\perp$.
Therefore, by parts (b) and (c) from 6.55, we have

$$
\begin{aligned}
P_U Tv &= P_U Tu + P_U Tw\\\\
&= P_U Tu\\\\
&= Tu\\\\
&= TP_U u\\\\
&= TP_U u + TP_U w\\\\
&= TP_U v.
\end{aligned}
$$

Hence $P_U T = TP_U$.

Conversely, suppose $P_U T = TP_U$.
Let $u \in U$.
Then

$$
Tu = TP_U u = P_U Tu \in U,
$$

Hence $U$ is invariant under $T$.
Let $w \in U^\perp$.
Then

$$
\begin{aligned}
Tw &= Tw - TP_U w = Tw - P_U Tw = (I - P_U)Tw = P_{U^\perp} Tw \in U^{\perp}
\end{aligned}
$$

where the last equality follows from Exercise 5.
Therefore $U^\perp$ is invariant under $T$.

## _Exercise 11_

Applying the Gram-Schmidt procedure to the basis $(1, 1, 0, 0), (1, 1, 1, 2)$ we get $\frac{1}{\sqrt{2}}(1, 1, 0, 0), \frac{1}{\sqrt{5}}(0, 0, 1, 2)$.
Using the formula from part (i) in 6.55 to calculate $P_U (1, 2, 3, 4)$, we get

$$
P_U (1, 2, 3, 4) = \frac{3}{2}(1, 1, 0, 0) + \frac{11}{5}(0, 0, 1, 2).
$$

## _Exercise 12_

Define $U$ by

$$
U = \\{p \in P_3(\mathbb{R}): p(0) = 0 \text{ and } p'(0)\\}.
$$

Note that $U$ is a subspace of $\mathcal{P}_3(\mathbb{R})$.
Let $u \in U$.
Since $p \in \mathcal{P}_3(\mathbb{R})$, we have

$$
p(x) = ax^3 + bx^2 + cx + d
$$

for some $a, b, c, d \in \mathbb{R}$.
$p(0) = 0$ and $p'(0) = 0$ now imply that $c = d = 0$ and so $U \subset \operatorname{span}(x^2, x^3)$.
Because $x^2, x^3 \in U$, it follows that $x^2, x^3$ is a basis of $U$.
Applying the Gram_Schmidt Procedure to this basis, we get

$$
\sqrt{5}x^2, 6\sqrt{7}x^3 - 5\sqrt{7}x^2.
$$

Now, using the formula from part(i) in 6.55 to get $P_U(2 + 3x)$, we get

$$
P_U(2 + 3x) = -\frac{203}{10}x^3 + 24x^2.
$$

_Exercise 13_

In this Exercise, I used the SymPy Python package to calculate the integrals necessary for the Gram-Schmidt Procedure on the basis $1, x, x^2, x^3, x^4, x^5$ of $\mathcal{P}_5(\mathbb{R})$ and to compute the polynomial $p$ with the formula in 6.55 (i).
I found the following

$$
p(x) = x^{5} \left(- \frac{72765}{8 \pi^{8}} + \frac{693}{8 \pi^{6}} + \frac{654885}{8 \pi^{10}}\right) + x^{3} \left(- \frac{363825}{4 \pi^{8}} - \frac{315}{4 \pi^{4}} + \frac{39375}{4 \pi^{6}}\right) + x \left(- \frac{16065}{8 \pi^{4}} + \frac{105}{8 \pi^{2}} + \frac{155925}{8 \pi^{6}}\right),
$$

which, if you assume $\pi = 3.14159265359$, is exactly what appers in 6.60.
Here is the code used:

```python
from sympy import *

x = Symbol('x')

def inner_product(f, g):
    return integrate(f*g, (x, -pi, pi))

def gs_procedure(basis):
    orthonormal_basis = []

    for j, v_j in enumerate(basis):
        e_j = v_j - sum(map(lambda e_k: inner_product(v_j, e_k) * e_k, orthonormal_basis[:j - 1]))
        e_j = e_j / sqrt(inner_product(e_j, e_j))
        orthonormal_basis.append(e_j)

    return orthonormal_basis

def project(func, orthonormal_basis):
    return sum(map(lambda e_j: inner_product(func, e_j) * e_j, orthonormal_basis))

orthonormal_basis = gs_procedure([1, x, x**2, x**3, x**4, x**5])

approx_sin = project(sin(x), orthonormal_basis)

p = collect(expand(approx_sin), x)
print(latex(p))
```
